theories/ValueOpts/ValueOpts.v
@@ -1,15 +1,13 @@
 Require Import CSet Le.
 
 Require Import Plus Util AllInRel Map LengthEq.
-Require Import CSet Val Var Env Equiv.Sim IL Fresh Annotation Coherence RenamedApart.
+Require Import CSet Val Var Env SimF IL Fresh Annotation Coherence RenamedApart.
 
-Require Import SetOperations Liveness Eqn SimF OptionR.
+Require Import SetOperations Liveness Eqn OptionR.
 
 Set Implicit Arguments.
 Unset Printing Records.
 Print Coercions.
-
-Qed.
 
 Inductive eqn_sound : list params -> list (set var) -> list eqns  (*params*set var*eqns*)
                       -> stmt -> stmt
@@ -46,16 +44,19 @@ Inductive eqn_sound : list params -> list (set var) -> list eqns  (*params*set v
     -> eqn_sound ZL Δ Γ (stmtLet x (Call f Y) s) (stmtLet x (Call f Y') s') Gamma
                 (ann1 (G,G') ang)
 | EqnFun ZL Δ Γ ΓF F F' t t'  Gamma Γ2 G G' angs angb
-  : length(ΓF) = length F 
-    -> length F = length F'
-    -> (forall n Z s Z' s' , get F n (Z, s) -> get F' n (Z', s') -> Z = Z')
-    -> (forall n Z s Z' s' EqS angn , get F n (Z, s) -> get F' n (Z', s')  -> get ΓF n EqS -> get angs n angn
-                                ->  eqn_sound (List.map fst F ++ ZL) ((List.map (fun _ => G) F) ++ Δ) (ΓF ++Γ)  s s' (EqS ∪ Γ2) angn)
-    -> eqn_sound (List.map fst F ++ ZL) ((List.map (fun _ => G) F) ++ Δ) (ΓF ++Γ)  t t' Gamma angb
-(*  -> eqns_freeVars EqS ⊆ G ++ of_list Z
-  -> eqns_freeVars Γ2  ⊆ G *)
-  -> entails Gamma Γ2
-  -> eqn_sound ZL Δ Γ (stmtFun F t) (stmtFun F' t') Gamma
+         (Len1:length(ΓF) = length F)
+         (Len2: length F = length F')
+         (ParamEq:forall n Z s Z' s' , get F n (Z, s) -> get F' n (Z', s') -> Z = Z')
+         (IndF:forall n Z s Z' s' EqS angn , get F n (Z, s) -> get F' n (Z', s')
+                                        -> get ΓF n EqS -> get angs n angn
+                                        -> eqn_sound (List.map fst F ++ ZL)
+                                                    ((List.map (fun _ => G) F) ++ Δ)
+                                                    (ΓF ++Γ)  s s' (EqS ∪ Γ2) angn)
+         (Indt:eqn_sound (List.map fst F ++ ZL) ((List.map (fun _ => G) F) ++ Δ) (ΓF ++Γ)  t t' Gamma angb)
+         (EqnFVF: forall n EqS Zs, get F n Zs -> get ΓF n EqS -> eqns_freeVars EqS ⊆ G ∪ of_list (fst Zs))
+         (EqnFV:eqns_freeVars Γ2  ⊆ G)
+         (Ent: entails Gamma Γ2)
+  : eqn_sound ZL Δ Γ (stmtFun F t) (stmtFun F' t') Gamma
               (annF (G,G') angs angb)
 | EqnUnsat ZL Δ Γ s s' Gamma ang
   : unsatisfiable Gamma
@@ -131,6 +132,8 @@ Proof.
   eapply map_1; eauto. eapply freeVars_Proper.
 Qed.
 
+Hint Resolve eqns_freeVars_incl : cset.
+
 Lemma eqns_freeVars_union Gamma Γ'
   : eqns_freeVars (Gamma ∪ Γ') [=] eqns_freeVars (Gamma) ∪ eqns_freeVars Γ'.
 Proof.
@@ -190,51 +193,47 @@ Proof.
   intros [A B]; hnf; intros. cset_tac.
 Qed.
 
+Lemma satisfies_agree E E' gamma
+  : satisfies E gamma
+    -> agree_on eq (Eqn.freeVars gamma) E E'
+    -> satisfies E' gamma.
+Proof.
+  intros. general induction gamma; simpl in *.
+  - erewrite !op_eval_agree; eauto with cset.
+  - erewrite !op_eval_agree; eauto with cset.
+  - eauto.
+Qed.
+
+Lemma satisfiesAll_agree E E' Gamma
+  : satisfiesAll E Gamma
+    -> agree_on eq (eqns_freeVars Gamma) E E'
+    -> satisfiesAll E' Gamma.
+Proof.
+  intros; hnf; intros.
+  eapply satisfies_agree; eauto using agree_on_incl with cset.
+Qed.
+
 Lemma satisfies_update_dead E gamma x v
 : satisfies E gamma
   -> x ∉ freeVars gamma
   -> satisfies (E[x <- v]) gamma.
-Admitted.
-(*
 Proof.
-  admit.
-Qed.
   intros.
-  destruct gamma; simpl in * |- *.
-  - inv H. symmetry in H2. symmetry in H1.
-    erewrite exp_eval_agree; try eapply H1.
-    symmetry.
-    erewrite exp_eval_agree; try eapply H2.
-    econstructor; reflexivity.
-    symmetry. eapply agree_on_update_dead; eauto.
-    cset_tac; intuition.
-    symmetry. eapply agree_on_update_dead; eauto.
-    cset_tac; intuition.
-  - inv H.
-    + symmetry in H2.
-      erewrite exp_eval_agree; try eapply H2. econstructor.
-      symmetry. eapply agree_on_update_dead; eauto.
-      cset_tac; intuition.
-    + symmetry in H1. symmetry in H2.
-      erewrite exp_eval_agree; try eapply H1.
-      erewrite exp_eval_agree; try eapply H2.
-      econstructor; reflexivity.
-      symmetry. eapply agree_on_update_dead; eauto.
-      cset_tac; intuition.
-      symmetry. eapply agree_on_update_dead; eauto.
-      cset_tac; intuition.
-  - eauto.
+  eapply satisfies_agree; eauto.
+  symmetry.
+  eapply agree_on_update_dead; eauto.
 Qed.
- *)
+
 Lemma satisfiesAll_add E gamma Gamma
   : satisfiesAll E {gamma ; Gamma}
     <-> satisfies E gamma /\ satisfiesAll E Gamma.
 Proof.
   split.
   intros H; split; hnf; intros; eapply H; cset_tac; intuition.
-  intros [A B]; hnf; intros. cset_tac; intuition.
+  intros [A B]; hnf; intros. cset_tac'.
   destruct H0; dcr; subst; eauto.
 Qed.
+
 (*
 Lemma satisfies_update_dead_list E gamma Z vl
 : length Z = length vl
@@ -297,16 +296,13 @@ Lemma eval_op_subst E y Y Z e
     op_eval E (subst_op (sid [Z <-- Y]) e).
 Proof.
   general induction e; simpl; eauto.
-  decide (v ∈ of_list Z).
-  eapply length_length_eq in H.
-  general induction H; simpl in * |- *; eauto.
-  symmetry in H0. monad_inv H0. simpl.
-  lud; eauto. eapply IHlength_eq; eauto.
-  cset_tac; intuition.
-  repeat rewrite lookup_set_update_not_in_Z; eauto.
-  erewrite IHe; eauto.
-  erewrite IHe1; eauto.
-  erewrite IHe2; eauto.
+  - eapply length_length_eq in H.
+    general induction H; simpl in * |- *; eauto.
+    symmetry in H0. monad_inv H0. simpl.
+    lud; eauto.
+  - erewrite IHe; eauto.
+  - erewrite IHe1; eauto.
+    erewrite IHe2; eauto.
 Qed.
 
 
@@ -321,7 +317,7 @@ Proof.
 Qed.
 
 
-    
+
 Lemma agree_on_onvLe_update_list {X} `{OrderedType.OrderedType X} (V V':onv X) Z vl
 : onvLe V V'
   -> onvLe (V [Z <-- vl]) (V' [Z <-- vl]).
@@ -393,8 +389,8 @@ Lemma entails_add' Gamma gamma Γ'
   -> entails Gamma {gamma; Γ'}.
 Proof.
   unfold entails; intros; dcr; intros.
-  - hnf; intros. cset_tac; intuition.
-    + eapply H0; cset_tac; intuition.
+  - hnf; intros. cset_tac'.
+    + eapply H0; cset_tac.
     + eapply H; eauto.
 Qed.
 
@@ -403,7 +399,8 @@ Lemma entails_monotonic_add Gamma Γ' gamma
 : entails Gamma Γ' -> entails (gamma ∪ Gamma) Γ'.
 Proof.
   unfold entails; intros; dcr.
-  - hnf; intros. eapply H. hnf; intros. eapply H0. cset_tac; intuition. eauto.
+  - hnf; intros. eapply H. hnf; intros. eapply H0.
+    cset_tac. eauto.
 Qed.
 
 Lemma entails_union_split Gamma Γ' Γ''
@@ -424,7 +421,7 @@ Lemma entails_union Gamma Γ' Γ''
 Proof.
   unfold entails, satisfiesAll.
   intros; dcr.
-  + intros. cset_tac. 
+  + intros. cset_tac.
 Qed.
 
 Lemma entails_add_single Gamma gamma Γ'
@@ -433,8 +430,8 @@ Lemma entails_add_single Gamma gamma Γ'
     -> entails Gamma {gamma; Γ'}.
 Proof.
   unfold entails; intros; dcr; intros.
-  - hnf; intros. cset_tac; intuition.
-    + eapply H0; cset_tac; intuition.
+  - hnf; intros. cset_tac'.
+    + eapply H0; cset_tac.
     + eapply H; eauto.
 Qed.
 
@@ -531,7 +528,7 @@ Lemma entails_union' Gamma Γ' Γ'' Γ'''
     -> entails Gamma (Γ''').
 Proof.
   intros; hnf; intros; hnf; intros.
-  rewrite H in H3. cset_tac.
+  rewrite H in H3. cset_tac'.
   - eapply H0; eauto.
   - eapply H1; eauto.
 Qed.
@@ -555,107 +552,100 @@ Lemma entails_eqns_trans Gamma e e' e''
     -> entails Gamma {EqnEq e e''}.
 Proof.
   intros. hnf; intros.
-  hnf; intros. cset_tac. hnf; intros. rewrite <- H2.
+  hnf; intros. cset_tac'. hnf; intros. rewrite <- H2.
   exploit (H1 _ H); eauto.
   exploit (H1 _ H0); eauto.
-  simpl in *. inv H3; inv H4; eauto using OptionR.option_R; try congruence.
+  etransitivity; eauto.
 Qed.
 
 
 Lemma entails_eqns_apx_refl e Gamma
   : entails Gamma {EqnApx e e}.
 Proof.
-  hnf; intros. hnf; intros. hnf; intros. cset_tac. rewrite <- H0.
+  hnf; intros. hnf; intros. hnf; intros.
+  cset_tac'. rewrite <- H0.
   reflexivity.
 Qed.
 
-(*
-Lemma satisfiesAll_subst V Gamma Γf Z EqS Y y bE G
+
+Lemma satisfiesAll_subst V Gamma Z EqS Y y bE G
 :  length Z = length Y
    -> eqns_freeVars EqS ⊆ G ∪ of_list Z
-   -> G ∩ of_list Z [=] ∅
    -> entails Gamma (subst_eqns (sid [Z <-- Y]) EqS)
    -> satisfiesAll V Gamma
    -> agree_on eq G V bE
-   -> ⎣y ⎦ = omap (op_eval V) Y
-   -> satisfiesAll bE Γf
+   -> omap (op_eval V) Y = ⎣y⎦
    -> satisfiesAll (bE [Z <-- List.map Some y]) EqS.
 Proof.
   revert_except EqS. pattern EqS. eapply set_induction; intros.
   - hnf; intros. eapply empty_is_empty_1 in H.
-    exfalso. rewrite H in H8. cset_tac; intuition.
-  - hnf; intros. eapply Add_Equal in H1. rewrite H1 in H10.
-    eapply add_iff in H10. destruct H10.
-    + hnf in H10; subst.
-      specialize (H5 V H6 (subst_eqn (sid [Z <-- Y]) gamma)). exploit H5.
-      eapply in_subst_eqns; eauto. rewrite H1. cset_tac; intuition.
-      hnf in X. destruct gamma. simpl in *. inv X.
-      * do 2 erewrite <- eval_exp_subst in X; eauto.
-        erewrite exp_eval_agree; [| |reflexivity].
-        erewrite exp_eval_agree with (e:=e'); [| |reflexivity].
-        eapply X.
-        eapply update_with_list_agree; eauto.
-        eapply agree_on_incl; eauto.
-        assert (EqnEq e e' ∈ s'). rewrite H1.
-        cset_tac; intuition.
-        exploit eqns_freeVars_incl; eauto. simpl in *.
-        rewrite H3 in X0.
-        rewrite <- (minus_union_set _ _ _ H4); eauto.
-        rewrite <- X0. eapply incl_minus_lr; cset_tac; intuition.
-        rewrite map_length. simpl in *.
-        exploit omap_length; eauto. congruence.
-        eapply update_with_list_agree; eauto.
-        eapply agree_on_incl; eauto.
-        assert (EqnEq e e' ∈ s'). rewrite H1.
-        cset_tac; intuition.
-        exploit eqns_freeVars_incl; eauto.
-        rewrite H3 in X0. simpl in X0.
-        rewrite <- (minus_union_set _ _ _ H4); eauto.
-        rewrite <- X0. eapply incl_minus_lr; cset_tac; intuition.
-        rewrite map_length. simpl in *.
-        exploit omap_length; eauto. congruence.
+    exfalso. rewrite H in H6. cset_tac; intuition.
+  - hnf; intros.
+    assert (LEN:❬Y❭ = ❬y❭). {
+      eapply omap_length; eauto.
+    }
+    eapply Add_Equal in H1. rewrite H1 in H8.
+    eapply add_iff in H8. destruct H8.
+    + hnf in H8; subst.
+      specialize (H4 V H5 (subst_eqn (sid [Z <-- Y]) gamma)).
+      exploit H4 as SAT.
+      eapply in_subst_eqns; eauto. rewrite H1. cset_tac.
+      hnf in SAT. destruct gamma. simpl in *.
+      * do 2 erewrite <- eval_op_subst in SAT; eauto.
+        erewrite op_eval_agree; [| |reflexivity].
+        erewrite op_eval_agree with (e:=e'); [| |reflexivity].
+        eapply SAT.
+        -- eapply update_with_list_agree; eauto with len.
+           eapply agree_on_incl; eauto.
+           assert (EqnEq e e' ∈ s') as IN. {
+             rewrite H1. cset_tac.
+           }
+           exploit eqns_freeVars_incl as FVI; eauto. simpl in *.
+           rewrite H3 in FVI. revert FVI; clear; cset_tac.
+        -- eapply update_with_list_agree; eauto with len.
+           eapply agree_on_incl; eauto.
+           assert (EqnEq e e' ∈ s') as IN. {
+             rewrite H1. cset_tac.
+           }
+           exploit eqns_freeVars_incl as FVI; eauto.
+           rewrite H3 in FVI. simpl in *.
+           revert FVI; clear; cset_tac.
       * simpl in * |- *.
-        do 2 erewrite <- eval_exp_subst in X; eauto.
-        erewrite exp_eval_agree; [| |reflexivity].
-        erewrite exp_eval_agree with (e:=e'); [| |reflexivity].
-        eapply X.
-        eapply update_with_list_agree; eauto.
-        eapply agree_on_incl; eauto.
-        assert (EqnApx e e' ∈ s'). rewrite H1.
-        cset_tac; intuition.
-        exploit eqns_freeVars_incl; eauto. simpl in *.
-        rewrite H3 in X0.
-        rewrite <- (minus_union_set _ _ _ H4); eauto.
-        rewrite <- X0. eapply incl_minus_lr; cset_tac; intuition.
-        rewrite map_length. simpl in *.
-        exploit omap_length; eauto. congruence.
-        eapply update_with_list_agree; eauto.
-        eapply agree_on_incl; eauto.
-        assert (EqnApx e e' ∈ s'). rewrite H1.
-        cset_tac; intuition.
-        exploit eqns_freeVars_incl; eauto.
-        rewrite H3 in X0. simpl in X0.
-        rewrite <- (minus_union_set _ _ _ H4); eauto.
-        rewrite <- X0. eapply incl_minus_lr; cset_tac; intuition.
-        rewrite map_length. simpl in *.
-        exploit omap_length; eauto. congruence.
+        do 2 erewrite <- eval_op_subst in SAT; eauto.
+        erewrite op_eval_agree; [| |reflexivity].
+        erewrite op_eval_agree with (e:=e'); [| |reflexivity]; eauto.
+        -- eapply update_with_list_agree; eauto with len.
+           eapply agree_on_incl; eauto.
+           assert (EqnApx e e' ∈ s') as IN. {
+             rewrite H1. clear; cset_tac.
+           }
+           exploit eqns_freeVars_incl as FVI; eauto. simpl in *.
+           rewrite H3 in FVI.
+           revert FVI; clear; cset_tac.
+        -- eapply update_with_list_agree; eauto with len.
+           eapply agree_on_incl; eauto.
+           assert (EqnApx e e' ∈ s') as IN. {
+             rewrite H1. cset_tac.
+           }
+           exploit eqns_freeVars_incl as FVI; eauto.
+           rewrite H3 in FVI. simpl in *.
+           revert FVI; clear; cset_tac.
       * simpl in *; eauto.
-    + rewrite H1 in H5.
+    + rewrite H1 in H4.
       eapply H; try eapply H7; eauto.
-      rewrite <- H3. rewrite H1.
-      rewrite eqns_freeVars_add'. cset_tac; intuition.
-      eapply entails_morphism_impl; eauto. reflexivity.
-      unfold flip. eapply subst_eqns_morphism_subset; eauto.
-      cset_tac; intuition.
+      * rewrite <- H3. rewrite H1.
+        rewrite eqns_freeVars_add'. cset_tac; intuition.
+      * setoid_rewrite <- incl_add' in H4; eauto.
 Qed.
- *)
+
 Lemma in_eqns_freeVars x gamma Gamma
   : x \In freeVars gamma
     -> gamma ∈ Gamma
     -> x \In eqns_freeVars Gamma.
-Proof. 
+Proof.
   intros. eapply eqns_freeVars_incl; eauto.
 Qed.
+
 (*
 Lemma satisfiesAll_update x Gamma V e e' y
 : x ∉ eqns_freeVars Gamma
@@ -740,7 +730,7 @@ Proof.
   - econstructor; eauto using entails_monotone.
   - econstructor; eauto using entails_monotone.
   - econstructor; eauto.
-    + rewrite <- H7; eauto.
+    + rewrite <- H2; eauto.
 Qed.
 
 
@@ -771,9 +761,10 @@ Lemma entails_inert_add x Γ2 Γ2'
     -> entails {x ; Γ2} {x ; Γ2'}.
 Proof.
   unfold entails; intros; dcr.
-  - hnf; intros. cset_tac; intuition.
-    eapply H; eauto. hnf; intros; eapply H0.
-    cset_tac; intuition.
+  - hnf; intros. cset_tac'.
+    + eapply H0. cset_tac.
+    + eapply H; eauto. hnf; intros; eapply H0.
+      cset_tac.
 Qed.
 
 Lemma entails_transitive Γ Γ' Γ''
@@ -862,37 +853,11 @@ Proof.
 Qed.
 (*
 Definition ArgRel' (Z:params ) (VL VL': list val) : Prop :=
-  
+
 (*  /\ satisfiesAll ([Z <-- List.map Some VL]) (EqS ∪ Gamma)*).
 
 Definition ParamRel' (Zb:params) (Z Z' : list var) : Prop :=
  *)
-
-
-Instance AR : PointwiseProofRelationF params:= {
-                                                ArgRelFP Z VL VL' := length Z = length VL /\ VL = VL';
-                                                ParamRelFP Z Z' Zb := Z = Z' /\ Zb = Z'
-                                              }.
-
-
-Lemma sim_let_op_apx X (IST:ILStateType X) r (L L':X) V V' x x' e e' s s'
-      (EQ: fstNoneOrR eq (op_eval V e) (op_eval V' e'))
-      (SIM: forall v, op_eval V e = Some v
-                 -> (sim r \3/ r) Sim (L, V [x <- ⎣ v ⎦], s) (L', V' [x' <- ⎣ v ⎦], s'))
-  : sim r Sim (L, V, stmtLet x (Operation e) s) (L', V', stmtLet x' (Operation e') s').
-Proof.
-  inv EQ.
-  -  pfold ; eapply SimErr;
-       [ | eapply star2_refl | ].
-     + apply result_none.  inversion 1.
-     + eapply let_op_normal. eauto.
-  -  pfold; eapply SimSilent; [ eapply plus2O
-                              | eapply plus2O
-                              | ].
-     eapply step_let_op; eauto. eauto.
-     eapply step_let_op.  eauto. eauto.
-     eapply SIM; eauto.
-Qed.
 
 Lemma satisfies_fstNoneOrR_apx V e e' :
   satisfies V (EqnApx e e') -> fstNoneOrR eq (op_eval V e) (op_eval V e').
@@ -900,69 +865,14 @@ Proof.
   intros. eauto.
 Qed.
 
-Lemma sim_cond_op_apx X (IST:ILStateType X) r (L L':X) V V' e e' s1 s1' s2 s2'
-      (EQ:  fstNoneOrR eq (op_eval V e) (op_eval V' e'))
-      (SIM1: forall v, op_eval V e = Some v -> val2bool v = true ->
-                  (sim r \3/ r) Sim (L, V, s1) (L', V', s1'))
-      (SIM2: forall v, op_eval V e = Some v -> val2bool v = false ->
-                  (sim r \3/ r) Sim (L, V, s2) (L', V', s2'))
-  : sim r Sim (L, V, stmtIf e s1 s2) (L', V', stmtIf e' s1' s2').
-Proof.
-  inv EQ.
-  - pfold; eapply SimErr;
-      [|eapply star2_refl|].
-    + apply result_none. inversion 1.
-    + eapply cond_normal. eauto.
-  -  case_eq (val2bool y); intros.
-     + pfold; eapply SimSilent; [ eapply plus2O; [|eapply filter_tau_nil_eq]
-                                | eapply plus2O; [|eapply filter_tau_nil_eq]
-                                | eapply SIM1; eauto];
-       eapply step_cond_true; eauto.    
-     + pfold; eapply SimSilent; [ eapply plus2O; [|eapply filter_tau_nil_eq]
-                                | eapply plus2O; [|eapply filter_tau_nil_eq]
-                                | eapply SIM2; eauto];
-       eapply step_cond_false; eauto.
-Qed.
-
-Lemma sim_return_apx X (IST:ILStateType X) r (L L':X) V V' e e' 
-  :fstNoneOrR eq (op_eval V e) (op_eval V' e') -> sim r Sim (L, V, stmtReturn e) (L', V', stmtReturn e').
-Proof.
-  intros. inv H.
-  - pfold; eapply SimErr; [|eapply star2_refl|].
-    + rewrite result_return. eauto.
-    + apply return_normal.
-  - pfold; eapply SimTerm; [|eapply star2_refl|eapply star2_refl| | ].
-    + rewrite! result_return. congruence.
-    + apply return_normal.
-    + apply return_normal.
-Qed.
-
-
-Lemma sim_let_call_apx X (IST:ILStateType X) r (L L':X) V V' x x' f Y Y' s s'
-      (EQ: fstNoneOrR eq  (omap (op_eval V) Y)  (omap (op_eval V') Y'))
-      (SIM: forall v, (sim r \3/ r) Sim (L, V [x <- ⎣ v ⎦], s) (L', V' [x' <- ⎣ v ⎦], s'))
-  : sim r Sim (L, V, stmtLet x (Call f Y) s) (L', V', stmtLet x' (Call f Y') s').
-Proof.
-  inv EQ.
-  - pfold. eapply SimErr; [|eapply star2_refl | ]; [ simpl  | ].
-    + rewrite !result_none; isabsurd; eauto.
-    + eapply let_call_normal; eauto.
-  - symmetry in H0, H. 
-    pfold; eapply SimExtern;
-      [ eapply star2_refl
-      | eapply star2_refl
-      | step_activated; eauto using step_let_call
-      | step_activated; eauto using step_let_call | |];
-      intros ? ? STEP; eapply let_call_inversion in STEP; dcr; subst; eexists; split; try eapply step_let_call; eauto; congruence.  
-Qed.
-
-Lemma onvLe_op_eval_some V V' e v
-  :onvLe V V' -> op_eval V e = ⎣ v ⎦ -> op_eval V' e = ⎣ v ⎦.
+Lemma onvLe_op_eval_some V V'
+  :onvLe V V' -> forall e v, op_eval V e = ⎣ v ⎦ -> op_eval V' e = ⎣ v ⎦.
 Proof.
   intros. general induction e; simpl in * |- * ; eauto using @fstNoneOrR.
   - rewrite H0. exploit H; eauto.
-  - monad_inv H0. rewrite EQ. simpl. rewrite (IHe V V' x); eauto.
-  - monad_inv H0. rewrite EQ1. rewrite EQ. simpl. erewrite IHe1; eauto. erewrite IHe2; simpl; eauto.
+  - monad_inv H0. rewrite EQ. simpl. erewrite (IHe V V' H _ EQ); eauto.
+  - monad_inv H0. rewrite EQ1. rewrite EQ. simpl.
+    erewrite IHe1; eauto. erewrite IHe2; simpl; eauto.
 Qed.
 
 
@@ -970,7 +880,7 @@ Lemma onvLe_fstNoneOrR_apx V V' e :
   onvLe V V' -> fstNoneOrR eq (op_eval V e) (op_eval V' e).
 Proof with simpl; eauto using @fstNoneOrR, @onvLe_op_eval_some.
   intros. case_eq (op_eval V e) ...
-  intros. erewrite onvLe_op_eval_some... 
+  intros. erewrite onvLe_op_eval_some...
 Qed.
 
 Lemma satisfies_EqnEq_on_update   (x:var) e V v:
@@ -985,7 +895,7 @@ Qed.
 
 
 
-Lemma op_eval_true_satisfies  V e v 
+Lemma op_eval_true_satisfies  V e v
         : op_eval V e = ⎣ v ⎦ -> val2bool v = true -> satisfies V (EqnEq (UnOp UnOpToBool e) (Con val_true)).
 Proof.
   intros. unfold satisfies. simpl. rewrite H. simpl. unfold option_lift1. rewrite H0. simpl. reflexivity.
@@ -999,15 +909,15 @@ Qed.
 
 Lemma onvLe_omap_op_eval_some V V' Y vl
  : onvLe V V' -> (omap (op_eval V) Y) = ⎣ vl ⎦ -> (omap (op_eval V') Y) = ⎣ vl ⎦.
-Proof.  
+Proof.
   intros.
-  case_eq (omap (op_eval V) Y); simpl; eauto.
-  intros. general induction Y; simpl in * |- *; eauto.
-  monad_inv H0. monad_inv H1.
-  rewrite EQ,EQ1. simpl. exploit IHY; eauto.
-  rewrite H0. erewrite onvLe_op_eval_some; simpl in * |- *; eauto.
-  congruence.
-Qed.  
+  general induction Y; simpl in * |- *; eauto.
+  monad_inv H0.
+  rewrite EQ, EQ1. simpl.
+  exploit (onvLe_op_eval_some H) as EV; eauto. rewrite EV.
+  simpl. erewrite IHY; eauto.
+  reflexivity.
+Qed.
 
 Lemma onvLe_omap_op_eval_fstNoneOrEq V V' Y
   : onvLe V V'
@@ -1019,7 +929,7 @@ Proof.
   reflexivity.
 Qed.
 (*
-Lemma satisfies_omap_op_eval_some Gamma Y Y' V vl 
+Lemma satisfies_omap_op_eval_some Gamma Y Y' V vl
   : entails Gamma (list_EqnApx Y Y')
     -> ❬Y❭ = ❬Y'❭
     -> satisfiesAll V Gamma
@@ -1031,7 +941,7 @@ Proof.
   case_eq (omap (op_eval V) Y); eauto.
   intros. length_equify. general induction H0; simpl in * |- *; eauto using fstNoneOrR.
   monad_inv H2. monad_inv H4. rewrite EQ0, EQ3. simpl. erewrite IHlength_eq; eauto.
-  - replace (op_eval V y) with ⎣x2⎦; simpl; eauto. 
+  - replace (op_eval V y) with ⎣x2⎦; simpl; eauto.
  *)
 
 
@@ -1056,7 +966,7 @@ Proof.
   unfold satisfies in *. rewrite H0 in H1. inv H1.
   symmetry in H3. eapply onvLe_op_eval_some in H3; eauto. eapply onvLe_op_eval_some in H0; eauto.
   rewrite H0,H3. reflexivity.
-Qed.            
+Qed.
 
 Lemma onvLe_op_eval_satisfiesAll V V' Y Y' v
   : onvLe V V'
@@ -1070,9 +980,9 @@ Proof.
   length_equify. general induction H0; simpl in * |- *;  eauto.
   - unfold list_EqnApx in H3. simpl in *. cset_tac.
   - unfold list_EqnApx in *. simpl in * |- *.
-    cset_tac.
-    + monad_inv H1.  rewrite <- H4. eapply onvLe_op_eval_satisfies; eauto.
-    + monad_inv H1.  eapply IHlength_eq; eauto. 
+    cset_tac'.
+    + monad_inv H1. rewrite <- H5. eapply onvLe_op_eval_satisfies; eauto.
+    + monad_inv H1. eapply IHlength_eq; eauto.
 Qed.
 
 
@@ -1090,328 +1000,230 @@ Qed.
 
 
 
-  
+
 (*
   omap_satisfies_list_EqnApx, omap_exp_eval_onvLe
 *)
-  
+
+
+Lemma sim_let_op_apx X (IST:ILStateType X) r (L L':X) V V' x x' e e' s s'
+      (EQ: fstNoneOrR eq (op_eval V e) (op_eval V' e'))
+      (SIM: forall v, op_eval V e = Some v
+                 -> (sim r \3/ r) Sim (L, V [x <- ⎣ v ⎦], s) (L', V' [x' <- ⎣ v ⎦], s'))
+  : sim r Sim (L, V, stmtLet x (Operation e) s) (L', V', stmtLet x' (Operation e') s').
+Proof.
+  inv EQ.
+  -  pfold ; eapply SimErr;
+       [ | eapply star2_refl | ].
+     + apply result_none.  inversion 1.
+     + eapply let_op_normal. eauto.
+  -  pfold; eapply SimSilent; [ eapply plus2O
+                              | eapply plus2O
+                              | ].
+     eapply step_let_op; eauto. eauto.
+     eapply step_let_op.  eauto. eauto.
+     eapply SIM; eauto.
+Qed.
+
+Lemma sim_cond_op_apx X (IST:ILStateType X) r (L L':X) V V' e e' s1 s1' s2 s2'
+      (EQ:  fstNoneOrR eq (op_eval V e) (op_eval V' e'))
+      (SIM1: forall v, op_eval V e = Some v -> val2bool v = true ->
+                  (sim r \3/ r) Sim (L, V, s1) (L', V', s1'))
+      (SIM2: forall v, op_eval V e = Some v -> val2bool v = false ->
+                  (sim r \3/ r) Sim (L, V, s2) (L', V', s2'))
+  : sim r Sim (L, V, stmtIf e s1 s2) (L', V', stmtIf e' s1' s2').
+Proof.
+  inv EQ.
+  - pfold; eapply SimErr;
+      [|eapply star2_refl|].
+    + apply result_none. inversion 1.
+    + eapply cond_normal. eauto.
+  -  case_eq (val2bool y); intros.
+     + pfold; eapply SimSilent; [ eapply plus2O; [|eapply filter_tau_nil_eq]
+                                | eapply plus2O; [|eapply filter_tau_nil_eq]
+                                | eapply SIM1; eauto];
+       eapply step_cond_true; eauto.
+     + pfold; eapply SimSilent; [ eapply plus2O; [|eapply filter_tau_nil_eq]
+                                | eapply plus2O; [|eapply filter_tau_nil_eq]
+                                | eapply SIM2; eauto];
+       eapply step_cond_false; eauto.
+Qed.
+
+Lemma sim_return_apx X (IST:ILStateType X) r (L L':X) V V' e e'
+  :fstNoneOrR eq (op_eval V e) (op_eval V' e') -> sim r Sim (L, V, stmtReturn e) (L', V', stmtReturn e').
+Proof.
+  intros. inv H.
+  - pfold; eapply SimErr; [|eapply star2_refl|].
+    + rewrite result_return. eauto.
+    + apply return_normal.
+  - pfold; eapply SimTerm; [|eapply star2_refl|eapply star2_refl| | ].
+    + rewrite! result_return. congruence.
+    + apply return_normal.
+    + apply return_normal.
+Qed.
+
+
+Lemma sim_let_call_apx X (IST:ILStateType X) r (L L':X) V V' x x' f Y Y' s s'
+      (EQ: fstNoneOrR eq  (omap (op_eval V) Y)  (omap (op_eval V') Y'))
+      (SIM: forall v, (sim r \3/ r) Sim (L, V [x <- ⎣ v ⎦], s) (L', V' [x' <- ⎣ v ⎦], s'))
+  : sim r Sim (L, V, stmtLet x (Call f Y) s) (L', V', stmtLet x' (Call f Y') s').
+Proof.
+  inv EQ.
+  - pfold. eapply SimErr; [|eapply star2_refl | ]; [ simpl  | ].
+    + rewrite !result_none; isabsurd; eauto.
+    + eapply let_call_normal; eauto.
+  - symmetry in H0, H.
+    pfold; eapply SimExtern;
+      [ eapply star2_refl
+      | eapply star2_refl
+      | step_activated; eauto using step_let_call
+      | step_activated; eauto using step_let_call | |];
+      intros ? ? STEP; eapply let_call_inversion in STEP; dcr; subst; eexists; split; try eapply step_let_call; eauto; congruence.
+Qed.
+
 Hint Resolve satisfies_fstNoneOrR_apx onvLe_fstNoneOrR_apx.
 
-Lemma sim_vopt r L L' V V' s s' ZL Δ Γ Gamma ang
+
+
+Instance PR : PointwiseProofRelationF (params*eqns):=
+  {
+    ArgRelFP := fun E E' '(Z,Γ2) VL VL' => length Z = length VL /\ VL = VL'
+    /\ exists Γ Y V, entails Γ (subst_eqns (sid [Z <-- Y]) Γ2)
+               /\ satisfiesAll V Γ /\ omap (op_eval V) Y = Some VL
+               /\ agree_on eq (eqns_freeVars Γ2 \ of_list Z) V E;
+    ParamRelFP := fun '(Z,_) Z' Zb => Z = Z' /\ Zb = Z'
+  }.
+
+Lemma sim_vopt r L L' V V' s s' ZL Δ ΓL Gamma ang
   : satisfiesAll V Gamma
-    -> eqn_sound ZL Δ Γ s s' Gamma ang
-    -> labenv_sim Sim (sim r) AR ZL L L'
+    -> eqn_sound ZL Δ ΓL s s' Gamma ang
+    -> labenv_sim Sim (sim r) PR (zip pair ZL ΓL) L L'
     -> renamedApart s ang
     -> eqns_freeVars Gamma ⊆ fst (getAnn ang)
     -> onvLe V V'
+    -> (forall n b G Γf, get L n b ->
+                get Δ n G ->
+                get ΓL n Γf ->
+                G ⊆ fst (getAnn ang) /\
+                eqns_freeVars Γf ⊆ G ∪ of_list (block_Z b) /\
+                agree_on eq G (F.block_E b) V)
     -> sim r Sim  (L,V, s) (L',V', s').
 Proof.
-  intros SAT EQN SIML REAPT FV OLE.
+  intros SAT EQN SIML REAPT FV OLE EEQ.
   general induction EQN; (try (now exfalso; eapply H; eauto))
   ; simpl; invt renamedApart; simpl in * |- *.
-  - exploit H; eauto. exploit H1; eauto; [cset_tac|].  eapply (sim_let_op_apx il_statetype_F). 
-    +  etransitivity; eauto.
+  - exploit H; eauto.
+    exploit H1; eauto; [cset_tac|].
+    eapply (sim_let_op_apx il_statetype_F).
+    + etransitivity; eauto.
     + intros. left. eapply IHEQN; eauto.
-      *  unfold satisfiesAll.  intros. cset_tac.
-         -- rewrite <- H5. eauto using satisfies_EqnEq_on_update.
-         -- rewrite <- H4. eapply (@satisfies_EqnEq_on_update x e' V v); eauto. eapply satisfies_fstNoneOrR_apx in H2.
-            rewrite H3 in H2.  inv H2. reflexivity.
-         --  exploit SAT; eauto. apply satisfies_update_dead; eauto.
-             intros X. apply H7. apply FV. eapply in_eqns_freeVars; eauto.
-      * pe_rewrite. rewrite! eqns_freeVars_add. simpl. rewrite H0, H8, FV. clear. cset_tac.
+      *  unfold satisfiesAll. intros. cset_tac'.
+         -- rewrite <- H12. eauto using satisfies_EqnEq_on_update.
+         -- rewrite <- H4.
+            eapply (@satisfies_EqnEq_on_update x e' V v); eauto.
+            eapply satisfies_fstNoneOrR_apx in H2.
+            rewrite H3 in H2. inv H2. reflexivity.
+         -- exploit SAT; eauto. apply satisfies_update_dead; eauto.
+            intros X. apply H7. apply FV. eapply in_eqns_freeVars; eauto.
+      * pe_rewrite. rewrite! eqns_freeVars_add. simpl.
+        rewrite H0, H8, FV. clear. cset_tac.
       * eapply agree_on_onvLe; eauto.
-  -  exploit H; eauto.  exploit H0; eauto; [cset_tac|].  eapply (sim_cond_op_apx il_statetype_F).
+      * intros. exploit EEQ; dcr; eauto.
+        pe_rewrite. do 2 try split; eauto with cset.
+        symmetry. eapply agree_on_update_dead; eauto.
+        symmetry; eauto.
+  -  exploit H; eauto.  exploit H0; eauto; [cset_tac|].
+     eapply (sim_cond_op_apx il_statetype_F).
      + etransitivity; eauto.
      + intros. left. eapply IHEQN1; clear IHEQN1 IHEQN2; eauto.
-       * apply satisfiesAll_add. eauto using  op_eval_true_satisfies.   
+       * apply satisfiesAll_add. eauto using  op_eval_true_satisfies.
        * rewrite eqns_freeVars_add. simpl. pe_rewrite. intros a0 A. cset_tac.
+       * pe_rewrite; eauto with cset.
      + intros. left. eapply IHEQN2; clear IHEQN1 IHEQN2; eauto.
        * apply satisfiesAll_add. eauto using op_eval_false_satisfies.
        * rewrite eqns_freeVars_add . pe_rewrite.  intros gamma A. cset_tac.
-  - eapply labenv_sim_app; eauto; simpl.
+       * pe_rewrite. eauto with cset.
+  - eapply labenv_sim_app; eauto using zip_get; simpl.
     intros; split; intros; eauto.
-    simpl in *.  destruct H7; subst. exists Yv; split; eauto.  eapply omap_exp_eval_onvLe; eauto.
-    exploit H4; eauto. eapply omap_satisfies_list_EqnApx; eauto.
+    assert (EV:omap (op_eval V) Y' = ⎣ Yv ⎦). {
+      exploit H4; eauto. eapply omap_satisfies_list_EqnApx; eauto.
+    }
+    simpl in *; dcr; subst.
+    exists Yv; repeat split; eauto using omap_exp_eval_onvLe.
+    exists Gamma, Y', V. repeat split; eauto.
+    exploit EEQ; eauto; dcr. simpl in *.
+    symmetry; eapply agree_on_incl; eauto.
+    rewrite H14; eauto. clear; cset_tac.
   - eapply (sim_return_apx il_statetype_F).
     exploit H; eauto. exploit H0; eauto; [cset_tac|]. etransitivity; eauto.
-  -  exploit H; eauto.   eapply (sim_let_call_apx il_statetype_F); eauto; simpl.
-     + case_eq (omap (op_eval V) Y); eauto using fstNoneOrR.
-       intros. etransitivity; eauto using  onvLe_omap_op_eval_fstNoneOrEq.
-       rewrite <- H3. eapply satisfies_omap_op_eval_fstNoneOrR; eauto.
-     + intros. simpl. left. eapply IHEQN; eauto.
-       * eauto using satisfiesAll_EqnEq_on_update.
-       * pe_rewrite. cset_tac.
-       * eauto using agree_on_onvLe.
+  - exploit H; eauto. eapply (sim_let_call_apx il_statetype_F); eauto; simpl.
+    + case_eq (omap (op_eval V) Y); eauto using fstNoneOrR.
+      intros. etransitivity; eauto using  onvLe_omap_op_eval_fstNoneOrEq.
+      rewrite <- H3. eapply satisfies_omap_op_eval_fstNoneOrR; eauto.
+    + intros. simpl. left. eapply IHEQN; eauto.
+      * eauto using satisfiesAll_EqnEq_on_update.
+      * pe_rewrite. cset_tac.
+      * eauto using agree_on_onvLe.
+      * intros. exploit EEQ; dcr; eauto.
+        pe_rewrite. do 2 try split; eauto with cset.
+        symmetry. eapply agree_on_update_dead; eauto.
+        symmetry; eauto.
   - pone_step. left. eapply IHEQN; eauto.
-    + eapply labenv_sim_extension_ptw; eauto with len. 
-      * intros. hnf. intros. simpl in * |- *. dcr. subst. inv_get.  eapply H3; eauto.
-        -- clear IHEQN H3 H5 r0. (* indexwise *)
-        -- exploit H12; eauto. 
-        -- admit.
-        -- exploit H1; eauto. subst.
-          eapply agree_on_onvLe_update_list. eauto.
-      * hnf. intros. simpl in *. subst. inv_get. exploit H1; eauto.
+    + rewrite zip_app; eauto with len.
+      eapply labenv_sim_extension_ptw; eauto with len.
+      * intros. hnf. intros. simpl in * |- *. dcr. subst. inv_get.
+        exploit H7; eauto.
+        eapply H; eauto.
+        -- assert (SAT2:satisfiesAll V Γ2). {
+             eapply Ent in SAT; eauto.
+           }
+           rewrite satisfiesAll_union; split.
+           ++ exploit EqnFVF; eauto.
+             edestruct H8; eauto; dcr. simpl in *.
+             eapply satisfiesAll_subst
+             with (G:=eqns_freeVars x0 \ of_list Z); eauto.
+             eauto with len.
+             eauto with cset.
+           ++ eapply satisfiesAll_agree; eauto.
+             eapply agree_on_update_list_dead; eauto.
+             ** edestruct H8; eauto; dcr.
+                rewrite EqnFV. eauto.
+        -- rewrite eqns_freeVars_union.
+           rewrite EqnFV. edestruct H8; eauto; dcr. simpl in *.
+           rewrite H14.
+           exploit EqnFVF as EQ; eauto.
+           rewrite EQ. simpl.
+           clear; cset_tac.
+        -- exploit ParamEq; dcr; eauto; subst.
+           eapply agree_on_onvLe_update_list. eauto.
+        -- intros. eapply get_app_cases in H16. destruct H16.
+           ++ inv_get. edestruct H8; try eapply H13; eauto; dcr. simpl in *.
+             rewrite H15. split; eauto with cset.
+             exploit EqnFVF; eauto.
+             rewrite get_app_lt in H14; eauto with len. inv_get. simpl in *.
+             rewrite H5; split; eauto.
+             eapply agree_on_update_list_dead; eauto with len.
+           ++ dcr; simpl in *. rewrite Len1 in *.
+             rewrite get_app_ge in H14; eauto with len.
+             rewrite get_app_ge in H15; eauto with len.
+             len_simpl.
+             exploit EEQ; eauto; dcr.
+             edestruct H8; try eapply H13; eauto; dcr.
+             rewrite H5. simpl. split. eauto with cset.
+             simpl in *. split; eauto.
+             eapply agree_on_update_list_dead; eauto.
+             rewrite H23. eauto.
+      * hnf. intros. simpl in *. subst. inv_get. exploit ParamEq; dcr; eauto.
     + pe_rewrite. eauto.
-
-        
-        eapply satisfies_omap_op_eval_fstNoneOrR; eauto. eapply onvLe_op_eval_satisfiesAll; eauto.
-        
-        Lemma onvLe_op_eval_satisfies V V' e e' v
-          : onvLe V V'
-            -> op_eval V e = Some v
-            -> satisfies V (EqnApx e e')
-            -> satisfies V' (EqnApx e e').
-        Proof.
-          intros.
-          unfold satisfies in *. rewrite H0 in H1. inv H1.
-          symmetry in H3. eapply onvLe_op_eval_some in H3; eauto. eapply onvLe_op_eval_some in H0; eauto.
-          rewrite H0,H3. reflexivity.
-Qed.            
-
-        Lemma onvLe_op_eval_satisfiesAll V V' Y Y' v
-          : onvLe V V'
-            -> ❬Y❭ = ❬Y'❭
-            -> (omap (op_eval V) Y) = Some v
-            -> satisfiesAll V (list_EqnApx Y Y')
-            -> satisfiesAll V' (list_EqnApx Y Y').
-        Proof.
-          intros.
-          unfold satisfiesAll in *. intros.
-          length_equify. general induction H0; simpl in * |- *;  eauto.
-          - unfold list_EqnApx in H3. simpl in *. cset_tac.
-          - unfold list_EqnApx in *. simpl in * |- *.
-            cset_tac.
-            + monad_inv H1.  rewrite <- H4. eapply onvLe_op_eval_satisfies; eauto.
-            + monad_inv H1.  eapply IHlength_eq; eauto. 
+    + intros. eapply get_app_cases in H2. destruct H2.
+      ++ inv_get. pe_rewrite. split; eauto.
+        exploit EqnFVF; eauto.
+        rewrite get_app_lt in H0; eauto with len. inv_get. simpl in *.
+        rewrite H1; split; eauto.
+      ++ dcr; simpl in *. rewrite Len1 in *.
+        rewrite get_app_ge in H0; eauto with len.
+        rewrite get_app_ge in H1; eauto with len.
+        len_simpl.
+        exploit EEQ; eauto; dcr.
+        pe_rewrite. split; eauto.
 Qed.
-
-
-
-  
-                                       
-             Lemma tmp V V' A :  onvLe V V' -> satisfiesAll V A -> satisfiesAll V' A.
-        Proof.
-          intros. unfold satisfiesAll. intros. unfold onvLe in H. exploit H0; eauto. destruct gamma; eauto.
-          - simpl. 
-
-
-          
-  - exploit H; eauto. exploit X; eauto. cset_tac; reflexivity. inv X0.
-    inv H2.
-    + pfold. econstructor 3; try eapply star2_refl; eauto. stuck2.
-    + pose proof H2. symmetry in H3. eapply exp_eval_onvLe in H3; eauto.
-      pfold. econstructor; try eapply plus2O.
-      econstructor; eauto using eq_sym. reflexivity.
-      econstructor; eauto using eq_sym. reflexivity.
-      left. eapply IHEQN; eauto.
-      * eapply satisfiesAll_update; eauto.
-      * {
-          eapply simL'_update; eauto.
-          - intros. hnf in H4.
-            hnf. destruct x0 as [[[ ?] ?] ?]. dcr.
-            repeat (split; eauto).
-            rewrite H10, H12. simpl. clear_all; cset_tac; intuition.
-            symmetry. eapply agree_on_update_dead.
-            intro. eapply H7. eauto.
-            symmetry; eauto.
-            symmetry. eapply agree_on_update_dead.
-            intro. eapply H7. eauto.
-            symmetry; eauto.
-          - intros; reflexivity.
-        }
-      * rewrite H10. simpl. rewrite eqns_freeVars_add2.
-        rewrite FV. simpl. rewrite H8. rewrite H0.
-        clear_all; cset_tac; intuition.
-      * hnf; intros. lud; eauto.
-  - exploit H; eauto. exploit X; eauto. cset_tac; reflexivity. inv X0.
-    inv H1.
-    + pfold. econstructor 3; try eapply star2_refl; eauto. stuck2.
-    + pose proof H1. symmetry in H2. eapply exp_eval_onvLe in H2; eauto.
-      pfold. case_eq (val2bool y); intros.
-(*      assert (not_entails Gamma (UnOp 0 e, Con val_false)). {
-        hnf; intros. eexists V; split; eauto.
-        intro. hnf in H8. simpl in *.
-        rewrite <- H4 in H8. inv H8.
-        cbv in H7. destruct y. congruence.
-        cases in H18. congruence. cbv in H18. congruence.
-      } *)
-      econstructor; try eapply plus2O.
-      econstructor; eauto using eq_sym. reflexivity.
-      econstructor; eauto using eq_sym. reflexivity.
-      left. eapply IHEQN1; try eapply H9; eauto.
-      * eapply satisfiesAll_add; split; eauto.
-        hnf; intros.
-        simpl. rewrite <- H0. unfold option_lift1. unfold comp; simpl.
-        rewrite H3; constructor. reflexivity.
-      * eapply simL'_update; eauto.
-        unfold BlockRel.
-        destruct x as [[[ ?] ?] ?]; simpl; intros; dcr.
-        repeat (split; eauto).
-        rewrite H12; eauto.
-        clear_all; reflexivity.
-      * rewrite eqns_freeVars_add. rewrite FV, H12.
-        simpl. rewrite H7. cset_tac; intuition.
-      * (* assert (not_entails Gamma (UnOp 0 e, Con val_true)). {
-          hnf; intros. eexists V; split; eauto.
-          intro. hnf in H8. simpl in *.
-          rewrite <- H4 in H8. inv H8.
-          cbv in H7. destruct y.
-          cases in H18. cbv in H18. congruence.
-          congruence. congruence.
-        } *)
-        econstructor; try eapply plus2O.
-        econstructor 3; eauto using eq_sym. reflexivity.
-        econstructor 3; eauto using eq_sym. reflexivity.
-        {
-          left. eapply IHEQN2; try eapply H13; eauto.
-          - eapply satisfiesAll_add; split; eauto.
-            hnf; intros. simpl. rewrite <- H0. unfold option_lift1.
-            unfold comp; simpl. rewrite H3. constructor. reflexivity.
-          - eapply simL'_update; eauto.
-            unfold BlockRel.
-            destruct x as [[[ ?] ?] ?]; simpl; intros; dcr.
-            repeat (split; eauto).
-            rewrite H13; eauto.
-            clear_all; reflexivity.
-          - rewrite eqns_freeVars_add; simpl.
-            rewrite FV, H7, H13. simpl. cset_tac; intuition.
-        }
-  - destruct (get_dec L (counted l)) as [[[bE bZ bs]]|].
-    (* hnf in H2. exploit H2; eauto. simpl in *. subst bZ. *)
-    decide (length bZ = length Y).
-    exploit H2; eauto. case_eq (omap (exp_eval V) Y); intros. Focus 2.
-    + pfold. econstructor 3; try eapply star2_refl. eauto. stuck2.
-    + pose proof H3.
-      eapply omap_satisfies_list_EqnApx in H4; eauto.
-      eapply omap_exp_eval_onvLe in H4; eauto.
-      pose proof H3.
-      eapply omap_satisfies_list_EqnApx in H5; eauto.
-      edestruct AIR5_length; try eassumption; dcr.
-      edestruct get_length_eq; try eassumption.
-      edestruct AIR5_nth as [?[? [?]]]; try eassumption; dcr.
-      simpl in *. repeat get_functional; subst.
-      inv H18. hnf in H21; simpl in H23; dcr; subst.
-      eapply sim_drop_shift. eapply H24; eauto.
-      hnf. simpl; repeat split.
-      exploit omap_length; eauto. unfold var in *. congruence.
-      eapply satisfiesAll_union; split; eauto.
-      symmetry in H5.
-      eapply (@satisfiesAll_subst V Gamma Γf); try eapply H5; eauto.
-      congruence.
-      symmetry; eauto.
-      eapply satisfiesAll_update_dead; eauto. rewrite map_length.
-      exploit omap_length; eauto. congruence.
-      rewrite <- H.
-      revert H H25; clear_all; cset_tac; intuition; exfalso; eauto.
-    + pfold. econstructor 3; try eapply star2_refl. eauto. stuck2; eauto.
-      get_functional; subst. simpl in *. congruence.
-    + pfold. econstructor 3; try eapply star2_refl. eauto. stuck2; eauto.
-  - simpl. exploit H; eauto. exploit X. cset_tac; reflexivity. inv X0; eauto.
-    inv H1.
-    + pfold. econstructor 3; try eapply star2_refl. simpl. congruence.
-      stuck2.
-    + pfold. econstructor 4; try eapply star2_refl. simpl.
-      erewrite <- exp_eval_onvLe in H0; eauto.
-      stuck2. stuck2.
-  - case_eq (omap (exp_eval V) Y); intros. Focus 2.
-    + pfold. econstructor 3; try eapply star2_refl. eauto.
-      stuck2.
-    + pose proof H2.
-      eapply omap_satisfies_list_EqnApx in H3; eauto.
-      eapply omap_exp_eval_onvLe in H3; eauto.
-      pfold. eapply sim'Extern; try eapply star2_refl.
-      * exists (ExternI f l 0); eexists; econstructor; eauto.
-      * pose proof H2. eapply omap_exp_eval_onvLe in H2; eauto.
-        eexists (ExternI f l 0); eexists; econstructor; eauto.
-      * { intros. inv H4.
-          eexists. econstructor; eauto.
-          - econstructor; eauto.
-            eapply omap_exp_eval_onvLe; eauto.
-            eapply omap_satisfies_list_EqnApx; eauto.
-          - left. eapply IHEQN; eauto.
-            + eapply satisfiesAll_update_dead_single; eauto.
-            + eapply simL'_update; eauto.
-              * unfold BlockRel'. intros. simpl in *.
-                unfold BlockRel' in *.
-                destruct x0 as [[[ ?] ?] ?]; simpl; intros; dcr.
-                repeat (split; eauto).
-                rewrite H12. rewrite H9. simpl. clear_all; cset_tac; intuition.
-                symmetry. eapply agree_on_update_dead. rewrite H9. eauto.
-                symmetry; eauto.
-                symmetry. eapply agree_on_update_dead. rewrite H9. eauto.
-                symmetry; eauto.
-              * intros; reflexivity.
-            + rewrite H12, FV; simpl. clear_all; cset_tac; intuition.
-            + hnf; intros; lud; eauto.
-        }
-      * { intros. inv H4.
-          eexists. econstructor; eauto.
-          - econstructor; eauto.
-            pose proof H2.
-            erewrite <- omap_exp_eval_onvLe in H5; eauto. congruence.
-          - left. eapply IHEQN; eauto.
-            + eapply satisfiesAll_update_dead_single; eauto.
-            + eapply simL'_update; eauto.
-              * unfold BlockRel. intros. simpl in *.
-                unfold BlockRel' in *.
-                destruct x0 as [[[ ?] ?] ?]; simpl; intros; dcr.
-                repeat (split; eauto).
-                rewrite H9, H12. simpl. clear_all; cset_tac; intuition.
-                symmetry. eapply agree_on_update_dead. rewrite H9. eauto.
-                symmetry; eauto.
-                symmetry. eapply agree_on_update_dead. rewrite H9. eauto.
-                symmetry; eauto.
-              * intros; reflexivity.
-            + rewrite FV, H12; simpl. clear_all; cset_tac; intuition.
-            + hnf; intros; lud; eauto.
-        }
-  - pfold. econstructor; try eapply plus2O.
-    econstructor; eauto. reflexivity.
-    econstructor; eauto. reflexivity.
-    simpl. left. eapply IHEQN2; eauto.
-    + eapply simL_mon; eauto. eapply simL_extension'; eauto.
-      * eapply simL'_update; eauto.
-        unfold BlockRel.
-        destruct x as [[[ ?] ?] ?]; simpl; intros; dcr.
-        repeat (split; eauto).
-        rewrite H5, H15; reflexivity.
-        clear_all; reflexivity.
-      * hnf; split; intros. hnf; intuition.
-        hnf in H2; dcr.
-        eapply IHEQN1; try eapply H10; eauto.
-        eapply simL'_update; eauto.
-        unfold BlockRel. intros.
-        destruct x as [[[ ?] ?] ?]; dcr. simpl in H2.
-        simpl. dcr.
-        assert (sEQ: s0 [=] s0 \ of_list Z). {
-          assert (s0 ∩ of_list Z [=] ∅).
-          rewrite <- H9. rewrite H15 in H17.
-          revert H9 H17; simpl; clear_all; cset_tac; intuition; exfalso; eauto.
-          rewrite <- (minus_union_set _ _ _ H2).
-          clear_all; cset_tac; intuition.
-        }
-        repeat (split; eauto).
-        rewrite H13. rewrite H17, H15; simpl. eapply incl_right.
-        rewrite sEQ. symmetry.
-        eapply update_with_list_agree_minus; eauto. rewrite map_length; eauto.
-        symmetry; eauto.
-        rewrite sEQ. symmetry.
-        eapply update_with_list_agree_minus; eauto. rewrite map_length; eauto.
-        symmetry; eauto.
-        congruence.
-        symmetry; eauto.
-        reflexivity.
-        rewrite H13; simpl. rewrite eqns_freeVars_union.
-        rewrite H, H0. clear_all; cset_tac; intuition.
-        subst. eapply agree_on_onvLe; eauto.
-      * hnf; split; eauto.
-      * hnf; intros.
-        simpl. split.
-        rewrite <- H9. clear_all; cset_tac; intuition.
-        split.
-        rewrite H15; reflexivity.
-        repeat (split; eauto using satisfiesAll_monotone; try reflexivity).
-    + rewrite FV, H15; reflexivity.
-Qed.
-
-Print Assumptions sim_vopt.
