configure.sh
@@ -46,5 +46,5 @@ RM=$(for pat in $(cat _blacklist); do echo "$SOURCES" | grep -e $pat ; done | so
 FILTERSOURCES=$(comm -23 <(echo "$SOURCES") <(echo "$RM"))
 echo "Removed due to blacklist:"
 echo "$RM"
-echo $(cat _CoqProject) src/lvc_plugin.ml4 src/smpl.ml4 $FILTERSOURCES  > Make
+echo $(cat _CoqProject) src/lvc_plugin.ml4 $FILTERSOURCES  > Make
 echo "Make generated."
